New solutions

gcd_sol.dfy
@@ -1,32 +1,116 @@
+/*
+   The greatest common divisor (gcd) of two natural numbers m and n is a number k such that
+    (a) k divides m; (b) k divides n; and (c) k is the largest number with these properties.
+
+   Define a recursive function that computes a gcd of two numbers using the following properties of gcd.
+   (a) gcd(n, n) == n
+   (b) gcd(m, n) == gcd(m-n, n) whenever m > n
+   (c) gcd(m, n) == gcd(m, n-m) whenever n > m
+*/
 function gcd(m: nat, n: nat): nat
-  requires m>=1;
-  requires n>=1;
-  decreases m+n;
-{ 
-  if (n==m) then n 
-  else if (m>n) then gcd(m-n, n) 
-  else gcd(m, n-m) 
+  requires m > 0 && n > 0;
+  decreases m + n;
+{
+  /* your code here */
+  if (m == n) then m
+  else if (m > n) then gcd(m - n, n)
+  else gcd(m, n - m)
+}
+/**
+   Specify and verify a function to compute gcd of m and n
+ */
+method GcdCalc(m: nat, n: nat) returns (res: nat)
+  requires m > 0 && n > 0;
+  ensures res == gcd(m, n);
+  // your spec here
+{
+  var n1, m1 := n, m;
+  while (n1 != m1)
+    decreases m1 + n1;
+    invariant m1 > 0 && n1 > 0;
+    invariant gcd(m, n) == gcd(m1, n1);
+  {
+    if (m1 < n1) {
+     n1 := n1 - m1;
+    } else {
+     m1 := m1 - n1;
+    }
+  }
+  assert(m1 == n1);
+  return n1;
 }
 
+
+
+
+
+
+
+
+
+
+
+
+
+
+
+
+
+
+
+
+
+
+/* function gcd(m: nat, n: nat): nat
+  requires n > 0 && m > 0;
+  decreases m + n;
+{
+  if (n==m) then n
+  else if (m>n) then gcd(m-n, n)
+  else gcd(m, n-m)
+}
+*/
+
+
+
+
+
+
+
+
+
+
+
+
+
+
+
+
+/*
 method GcdCal(m: nat, n: nat) returns (res: nat)
-  requires m>=1;
-  requires n>=1;
   ensures res == gcd(m, n);
-{ 
+{
   var m1: nat, n1: nat := m, n;
-  while (m1!=n1) 
-    invariant m1 >= 1;
-    invariant n1 >= 1;
-    invariant gcd(m1, n1) == gcd (m, n)
-    decreases m1+n1
-  {  
-    if (m1>n1) { 
-      m1 := m1-n1; 
-    } 
-    else { 
-      n1 := n1-m1; 
+
+  while (m1!=n1)
+  {
+    if (m1>n1) {
+      m1 := m1-n1;
+    }
+    else {
+      n1 := n1-m1;
     }
  }
  return m1;
 }
+ */
 
+
+
+
+
+
+
+
+
+/* gcd lemma: use gcd(m, n) = gcd(n1, m1) */
